Engine/PikeEquiv.v
@@ -5,7 +5,7 @@ Import ListNotations.
 
 From Linden Require Import Regex Chars Groups.
 From Linden Require Import Tree Semantics BooleanSemantics.
-From Linden Require Import NFA PikeTree PikeVMSeen PikeSubset.
+From Linden Require Import NFA PikeTreeSeen PikeVMSeen PikeSubset.
 From Warblre Require Import Base RegExpRecord.
 
 
